spectec/isabelle_type_safety_proof/Context_Store_Agreement.thy
@@ -1,0 +1,113 @@
+ theory Context_Store_Agreement
+	imports Main isabelle_reference_output_wasm2 
+begin
+
+definition t_inst_match :: "res_context \<Rightarrow> res_context \<Rightarrow> bool" where
+  "t_inst_match C C' \<equiv> context_TYPES C = context_TYPES C' \<and>
+                       context_FUNCS C = context_FUNCS C' \<and>
+                       context_GLOBALS C = context_GLOBALS C' \<and>
+                       context_TABLES C = context_TABLES C' \<and>
+                       context_MEMS C = context_MEMS C' \<and>
+                       context_ELEMS C = context_ELEMS C' \<and>
+                       context_DATAS C = context_DATAS C'"
+
+lemma t_inst_match_is:
+  assumes "t_inst_match C1 C2"
+  shows "\<exists>a b c. C2 = \<lparr> context_TYPES = context_TYPES C1,
+                       context_FUNCS = context_FUNCS C1,
+                       context_GLOBALS = context_GLOBALS C1,
+                       context_TABLES = context_TABLES C1,
+                       context_MEMS = context_MEMS C1,
+                       context_ELEMS = context_ELEMS C1,
+                       context_DATAS = context_DATAS C1,
+                       context_LOCALS = a,
+                       LABELS = b,
+                       context_RETURN = c \<rparr>"
+  by (metis (full_types) assms unit.exhaust res_context.surjective t_inst_match_def)
+
+
+
+lemma blocktype_ok_agree:
+  assumes "Blocktype_ok C' bt tf"
+    "Moduleinst_ok s (frame_MODULE f) C"
+    "t_inst_match C C'"
+  shows "fun_blocktype (mk_state s f) bt = tf"
+  using assms
+proof(induction C' bt tf rule:Blocktype_ok.induct)
+  case (Blocktype_ok__valtype C valtype_opt)
+  then show ?case 
+  proof (cases valtype_opt)
+    case None
+    then show ?thesis using Blocktype_ok__valtype fun_blocktype.domintros 
+       fun_blocktype.psimps by auto
+  next
+    case (Some a)
+    then show ?thesis using Blocktype_ok__valtype fun_blocktype.domintros
+fun_blocktype.psimps by auto
+  qed
+next
+  case (Blocktype_ok__typeidx v_typeidx C' t_1_lst t_2_lst)
+  then have sametypes: "context_TYPES C' = context_TYPES C" using t_inst_match_def by simp
+  show ?case using Blocktype_ok__typeidx(5,1,2,3,4,6) fun_blocktype.domintros(3) fun_blocktype.psimps(3)
+      fun_type.domintros fun_type.psimps sametypes
+  proof (induction s "frame_MODULE f" C rule:Moduleinst_ok.induct)
+    case (mk_Moduleinst_ok functype_lst globaladdr_lst globaltype_lst s funcaddr_lst 
+          functype_F_lst memaddr_lst memtype_lst tableaddr_lst tabletype_lst exportinst_lst 
+          dataaddr_lst datatype_lst elemaddr_lst elemtype_lst)
+    then have "TYPES (frame_MODULE f) ! proj_uN_0 v_typeidx = context_TYPES C' ! proj_uN_0 v_typeidx"
+      by (metis moduleinst.select_convs(1) res_context.select_convs(1))
+    then show ?case using mk_Moduleinst_ok by metis
+  qed
+qed
+
+lemma list_all2_nth:
+  assumes "list_all2 P l1 l2" "l1 ! k = x1" "l2 ! k = x2" "k < length l1"
+  shows "P x1 x2" 
+  using assms 
+proof (induction l1 arbitrary: l2 k)
+  case Nil 
+  then show ?case
+    by simp
+  note outer = Nil
+next
+  case (Cons a l1)
+  note outer = Cons
+  then show ?case 
+  proof (cases l2)
+    case Nil
+    then show ?thesis using outer by simp
+  next
+    case (Cons b list)
+    then show ?thesis 
+    proof (cases k)
+      case 0
+      then show ?thesis using outer Cons by simp
+    next
+      case (Suc nat)
+      then show ?thesis using outer Cons by auto
+    qed
+  qed
+qed
+
+lemma context_funcs_agree:
+  assumes "context_FUNCS C' ! x = tf" 
+          "x < length (context_FUNCS C')"
+          "fun_funcaddr (mk_state s f) ! x = y"
+          "wf_store s" 
+          "Moduleinst_ok s (frame_MODULE f) C" 
+          "t_inst_match C C'"
+        shows "Externaddr_ok s (externaddr_FUNC y) (FUNC tf)"
+proof - 
+  have eqfuncs: "context_FUNCS C' = context_FUNCS C" using assms t_inst_match_def by simp
+  show ?thesis using assms(5,1,2,3,4,6) eqfuncs
+    proof (induction s "frame_MODULE f" C rule:Moduleinst_ok.induct)
+      case (mk_Moduleinst_ok functype_lst globaladdr_lst globaltype_lst s funcaddr_lst 
+              functype_F_lst memaddr_lst memtype_lst tableaddr_lst tabletype_lst exportinst_lst 
+              dataaddr_lst datatype_lst elemaddr_lst elemtype_lst)
+      show ?case using mk_Moduleinst_ok(30,27,28,29,33) fun_funcaddr.psimps fun_funcaddr.domintros
+        list_all2_nth[OF mk_Moduleinst_ok(5)]
+        by (metis mk_Moduleinst_ok.hyps(4) moduleinst.select_convs(2) res_context.select_convs(2))
+    qed
+  qed
+
+end
